prove some admitted lemmas

aneris/examples/reliable_communication/lib/repdb/model.v
@@ -38,8 +38,7 @@ Section ValidStates.
   Definition mem_dom (M : gmap Key (option write_event)) := DB_keys = dom M.
 
   Definition mem_we_key (M : gmap Key (option write_event)) :=
-    ∀ k (we : write_event), k ∈ dom M →
-                            M !! k = Some (Some we) → we.(we_key) = k.
+    ∀ k we, M !! k = Some (Some we) → we.(we_key) = k.
 
   Definition mem_log_coh (L : wrlog) (M : gmap Key (option write_event)) :=
     ∀ k, k ∈ dom M → M !! k = Some (at_key k L).
@@ -48,16 +47,16 @@ Section ValidStates.
     ∀ k we, at_key k L = Some we → M !! k = Some (Some we).
 
  Definition mem_serializable_vals (M : gmap Key (option write_event)) :=
-    ∀ k we, k ∈ dom M → M !! k = Some (Some we) →
-            Serializable DB_serialization we.(we_val).
+    ∀ k we, M !! k = Some (Some we) → Serializable DB_serialization we.(we_val).
 
   Definition allocated_in_mem (L : wrlog) (M : gmap Key (option write_event)) :=
     ∀ l k wel, l ≤ₚ L → at_key k l = Some wel →
                ∃ weL, M !! k = Some (Some weL) ∧ wel ≤ₜ weL.
 
+  (* why are scopes screwed up here!? *)
   Definition log_events (L : wrlog) :=
-    ∀ (i : nat), 0 <= i → i < List.length L →
-         ∃ we, List.nth_error L i = Some we ∧ i = we.(we_time) ∧ we.(we_key) ∈ DB_keys ∧
+    ∀ (i : nat), (i < List.length L)%nat →
+         ∃ we, L !! i = Some we ∧ i = we.(we_time) ∧ we.(we_key) ∈ DB_keys ∧
                  Serializable DB_serialization we.(we_val).
 
   Record valid_state (L : wrlog) (M : gmap Key (option write_event)) : Prop :=
@@ -77,50 +76,158 @@ Section ValidStates.
     split; rewrite /mem_dom /mem_we_key /mem_log_coh /in_log_mem_some_coh
                    /mem_serializable_vals /allocated_in_mem /log_events.
     - by rewrite dom_gset_to_gmap.
-    - intros ? ? ? Habs. apply lookup_gset_to_gmap_Some in Habs. naive_solver.
+    - intros ? ? Habs. apply lookup_gset_to_gmap_Some in Habs. naive_solver.
     - intros k Hy2. apply lookup_gset_to_gmap_Some. rewrite dom_gset_to_gmap in Hy2. naive_solver.
     - intros k we He. naive_solver.
-    - intros k we Hk Hnone. apply lookup_gset_to_gmap_Some in Hnone. naive_solver.
+    - intros k we Hnone. apply lookup_gset_to_gmap_Some in Hnone. naive_solver.
     - intros l k wel Hpre Hsm. destruct Hpre as (h2 & Hpre).
       symmetry in Hpre. apply app_eq_nil in Hpre. naive_solver.
-    - intros i Hi0 Hin. rewrite nil_length in Hin. by lia.
+    - intros i Hin. rewrite nil_length in Hin. by lia.
   Qed.
 
   Lemma log_events_serializable L M :
     valid_state L M →
     ∀ (we : write_event),
-    In we L →
+    we ∈ L →
     Serializable
      (prod_serialization
         (prod_serialization string_serialization DB_serialization)
         int_serialization) ($ we).
   Proof.
-  Admitted.
+    intros Hvs we Hwe.
+    destruct we as [k v t].
+    apply (_ : _ → _ → Serializable (prod_serialization _ _) (_, _)); last apply _.
+    apply (_ : _ → _ → Serializable (prod_serialization _ _) (_, _)); first apply _.
+    apply elem_of_list_lookup_1 in Hwe as [i Hiwe].
+    destruct (DB_GSTV_log_events _ _ Hvs i) as (?&Hi&?&?&?);
+      first by eapply lookup_lt_is_Some_1; eauto.
+    rewrite Hi in Hiwe; simplify_eq; done.
+  Qed.
+
+
+  (* TODO: MOVE *)
+  Lemma prefix_of_snoc {A} x (l1 l2 : list A) : l1 ≤ₚ (l2 ++ [x]) → l1 = l2 ++ [x] ∨ l1 ≤ₚ l2.
+  Proof.
+    intros [k Hk]. destruct k as [|y k _] using rev_ind .
+    - rewrite app_nil_r in Hk; by left.
+    - rewrite assoc in Hk. apply app_inj_2 in Hk as [? ?]; last done.
+      right; eexists; done.
+  Qed.
+
+  (* TODO: MOVE *)
+  Lemma at_key_elem_of k l we : at_key k l = Some we → we ∈ l.
+  Proof. intros ?; eapply elem_of_list_filter; apply last_Some_elem_of; done. Qed.
+
+(* TODO: MOVE *) (* again scope is screwed up! *)
+  Lemma lt_TM_lt we we' : (we_time we < we_time we')%nat → we ≤ₜ we'.
+  Proof. rewrite /TM_lt /=; by left. Qed.
+
+  Lemma log_events_state_update (lM : wrlog) wev :
+    wev.(we_key) ∈ DB_keys →
+    wev.(we_time) = length lM →
+    Serializable DB_serialization wev.(we_val) →
+    log_events lM ->
+    log_events (lM ++ [wev]).
+  Proof.
+    intros ??? HLE i. rewrite app_length /=. intros Hi.
+    destruct (decide (i = length lM)) as [->|].
+    + rewrite lookup_app_r; last done.
+      rewrite Nat.sub_diag /=.
+      eexists _; done.
+    + destruct (HLE i) as (?&Hi'&?&?&?); first lia.
+      eexists; split; last done.
+      rewrite lookup_app_l; first done.
+      apply lookup_lt_is_Some_1; eauto.
+  Qed.
 
   Lemma valid_state_update (lM : wrlog) (kvsMG : gmap Key (option write_event)) wev :
     wev.(we_key) ∈ DB_keys →
-    wev.(we_time) = (length lM : Time) →
+    wev.(we_time) = length lM →
     Serializable DB_serialization wev.(we_val) →
     valid_state lM kvsMG ->
     valid_state (lM ++ [wev]) (<[wev.(we_key) := Some wev]> kvsMG).
-  Proof. Admitted.
+  Proof.
+    intros Hwevk Hwevt Hwevser Hvs.
+    split.
+    - rewrite /mem_dom dom_insert_L subseteq_union_1_L; first apply Hvs.
+      erewrite <- DB_GSTV_mem_dom; last done.
+      set_solver.
+    - intros k we.
+      destruct (decide (k = we_key wev)) as [->|].
+      { rewrite lookup_insert; intros ?; simplify_eq; done. }
+      rewrite lookup_insert_ne; last done.
+      apply Hvs; done.
+    - intros k. rewrite dom_insert elem_of_union elem_of_singleton. intros Hk.
+      destruct (decide (k = we_key wev)) as [->|].
+      { rewrite lookup_insert at_key_snoc_some; done. }
+      destruct Hk as [->|Hk]; first done.
+      rewrite lookup_insert_ne; last done.
+      rewrite at_key_snoc_none; last done.
+      apply Hvs; done.
+    - intros k we.
+      destruct (decide (k = we_key wev)) as [->|].
+      + rewrite lookup_insert at_key_snoc_some; last done; intros ?; simplify_eq; done.
+      + rewrite lookup_insert_ne; last done.
+        rewrite at_key_snoc_none; last done.
+        apply Hvs.
+    - intros k we.
+      destruct (decide (k = we_key wev)) as [->|].
+      + rewrite lookup_insert; intros ?; simplify_eq; done.
+      + rewrite lookup_insert_ne; last done. apply Hvs.
+    - intros l k wel Hl Hklwel.
+      destruct (decide (k = we_key wev)) as [->|].
+      + rewrite lookup_insert. eexists; split; first done.
+        apply prefix_of_snoc in Hl as [->|Hl].
+        { rewrite at_key_snoc_some in Hklwel; last done; simplify_eq.
+          by right. (* this is weird; need to prove the Reflexive instance for ≤ₜ *) }
+        assert (∃ i, lM !! i = Some wel) as [i Hi].
+        { apply elem_of_list_lookup.
+          eapply elem_of_prefix; last done.
+          eapply at_key_elem_of; done. }
+        apply lt_TM_lt.
+        destruct (DB_GSTV_log_events _ _ Hvs i) as (?&Hi'&?&?&?);
+          first by apply lookup_lt_is_Some_1; eauto.
+        rewrite /TM_lt /=.
+        rewrite Hi in Hi'; simplify_eq.
+        rewrite Hwevt.
+        apply lookup_lt_is_Some_1; eauto.
+      + rewrite lookup_insert_ne; last done.
+        apply prefix_of_snoc in Hl as [->|Hl].
+        { rewrite at_key_snoc_none in Hklwel; last done; simplify_eq.
+          eapply Hvs; done. }
+        eapply Hvs; done.
+    - apply log_events_state_update; [done|done|done|apply Hvs].
+  Qed.
 
-  Lemma valid_state_log_no_dup lM mM:
-    valid_state lM mM ->
-    NoDup lM.
-  Proof. Admitted.
+  Lemma log_events_no_dup lM : log_events lM → NoDup lM.
+  Proof.
+    intros HLE.
+    apply (NoDup_fmap_1 we_time).
+    assert (we_time <$> lM = seq 0 (length lM)) as ->; last apply NoDup_seq.
+    apply list_eq.
+    intros i.
+    destruct (decide (i < length lM)%nat); last first.
+    { rewrite lookup_seq_ge; last lia.
+      rewrite list_lookup_fmap lookup_ge_None_2; first done. by apply Nat.nlt_ge. }
+    rewrite lookup_seq_lt /=; last done.
+    destruct (HLE i) as (?&Hi&Hit&?&?); first done.
+    rewrite list_lookup_fmap Hi /= -Hit //.
+  Qed.
+
+  Lemma valid_state_log_no_dup lM mM: valid_state lM mM -> NoDup lM.
+  Proof. intros Hvs; apply log_events_no_dup; apply Hvs. Qed.
 
  (** Local Validity. *)
   Definition mem_dom_local (M : gmap Key val) := dom M ⊆ DB_keys.
 
   Definition in_mem_log_some_coh_local (L : wrlog) (M : gmap Key val) :=
-    ∀ k v, k ∈ dom M → M !! k = Some v → ∃ we, at_key k L = Some we ∧ we.(we_val) = v.
+    ∀ k v, M !! k = Some v → ∃ we, at_key k L = Some we ∧ we.(we_val) = v.
 
   Definition in_mem_log_none_coh_local (L : wrlog) (M : gmap Key val) :=
     ∀ k, M !! k = None → at_key k L = None.
 
   Definition mem_serializable_vals_local (M : gmap Key val) :=
-    ∀ k v, k ∈ dom M → M !! k = Some v → Serializable DB_serialization v.
+    ∀ k v, M !! k = Some v → Serializable DB_serialization v.
 
   Definition in_log_mem_some_coh_local (L : wrlog) (M : gmap Key val) :=
     ∀ we, at_key we.(we_key) L = Some we →  M !! we.(we_key) = Some we.(we_val).
@@ -129,8 +236,7 @@ Section ValidStates.
     ∀ k, at_key k L = None → M !! k = None.
 
   Definition allocated_in_mem_local (L : wrlog) (M : gmap Key val) :=
-    ∀ l k we1, l ≤ₚ L → at_key k l = Some we1 →
-               ∃ we2, M !! k = Some we2.(we_val) ∧ we1 ≤ₜ we2.
+    ∀ l k we1, l ≤ₚ L → at_key k l = Some we1 → ∃ we2, M !! k = Some we2.(we_val) ∧ we1 ≤ₜ we2.
 
   Record valid_state_local (L : wrlog) (M : gmap Key val) : Prop :=
     {
@@ -149,24 +255,78 @@ Section ValidStates.
     split; rewrite /mem_dom_local /in_mem_log_some_coh_local /in_mem_log_none_coh_local
                     /mem_serializable_vals_local /in_log_mem_some_coh_local /in_log_mem_none_coh_local
                   /allocated_in_mem_local /log_events;  try set_solver.
-    - intros i Hi0 Hin. rewrite nil_length in Hin. by lia.
+    - intros i Hin. rewrite nil_length in Hin. by lia.
     - intros l k we1 Hpre.
       destruct Hpre as (h2 & Hpre).
       symmetry in Hpre. apply app_eq_nil in Hpre. naive_solver.
   Qed.
 
-  Lemma valid_state_local_update
-        (lM : wrlog) (kvsMG : gmap Key val) wev :
+  Lemma valid_state_local_update (lM : wrlog) (kvsMG : gmap Key val) wev :
     wev.(we_key) ∈ DB_keys →
-    wev.(we_time) = (length lM : Time) →
+    wev.(we_time) = length lM →
     Serializable DB_serialization wev.(we_val) →
     valid_state_local lM kvsMG ->
     valid_state_local (lM ++ [wev]) (<[wev.(we_key):= wev.(we_val)]> kvsMG).
-  Proof. Admitted.
+  Proof.
+    intros Hwevk Hwevt Hwevser Hvs.
+    split.
+    - apply log_events_state_update; [done|done|done|apply Hvs].
+    - intros k; rewrite dom_insert elem_of_union elem_of_singleton; intros [->|Hk]; first done.
+      apply Hvs; done.
+    - intros k v.
+      destruct (decide (k = we_key wev)) as [->|].
+      { rewrite lookup_insert; intros; simplify_eq; done. }
+      rewrite lookup_insert_ne; last done. apply Hvs.
+    - intros k v.
+      destruct (decide (k = we_key wev)) as [->|].
+      { rewrite lookup_insert; intros; simplify_eq.
+        rewrite at_key_snoc_some; eauto. }
+      rewrite lookup_insert_ne; last done.
+      rewrite at_key_snoc_none; last done.
+      apply Hvs.
+    - intros k.
+      destruct (decide (k = we_key wev)) as [->|].
+      { rewrite lookup_insert; done. }
+      rewrite lookup_insert_ne; last done.
+      rewrite at_key_snoc_none; last done.
+      apply Hvs.
+    - intros we.
+      destruct (decide (we_key we = we_key wev)) as [->|].
+      { rewrite at_key_snoc_some; last done. rewrite lookup_insert; intros; simplify_eq; done. }
+      rewrite at_key_snoc_none; last done.
+      rewrite lookup_insert_ne; last done.
+      apply Hvs.
+    - intros k.
+      destruct (decide (k = we_key wev)) as [->|].
+      { rewrite at_key_snoc_some; done. }
+      rewrite lookup_insert_ne; last done.
+      rewrite at_key_snoc_none; last done.
+      apply Hvs.
+    - intros l k wel Hl Hklwel.
+      destruct (decide (k = we_key wev)) as [->|].
+      + rewrite lookup_insert. eexists; split; first done.
+        apply prefix_of_snoc in Hl as [->|Hl].
+        { rewrite at_key_snoc_some in Hklwel; last done; simplify_eq.
+          by right. (* this is weird; need to prove the Reflexive instance for ≤ₜ *) }
+        assert (∃ i, lM !! i = Some wel) as [i Hi].
+        { apply elem_of_list_lookup.
+          eapply elem_of_prefix; last done.
+          eapply at_key_elem_of; done. }
+        apply lt_TM_lt.
+        destruct (DB_LSTV_log_events _ _ Hvs i) as (?&Hi'&?&?&?);
+          first by apply lookup_lt_is_Some_1; eauto.
+        rewrite /TM_lt /=.
+        rewrite Hi in Hi'; simplify_eq.
+        rewrite Hwevt.
+        apply lookup_lt_is_Some_1; eauto.
+      + rewrite lookup_insert_ne; last done.
+        apply prefix_of_snoc in Hl as [->|Hl].
+        { rewrite at_key_snoc_none in Hklwel; last done; simplify_eq.
+          eapply Hvs; done. }
+        eapply Hvs; done.
+  Qed.
 
-  Lemma valid_state_local_log_no_dup lM mM:
-    valid_state_local lM mM ->
-    NoDup lM.
-  Proof. Admitted.
+  Lemma valid_state_local_log_no_dup lM mM: valid_state_local lM mM -> NoDup lM.
+  Proof. intros Hvs; apply log_events_no_dup; apply Hvs. Qed.
 
 End ValidStates.
